theory/rBPFSem.thy
@@ -99,6 +99,16 @@ definition eval_jmp :: "condition \<Rightarrow> dst_ty \<Rightarrow> snd_op \<Ri
 )"
 
 
+definition eval_store :: "memory_chunk \<Rightarrow> dst_ty \<Rightarrow> snd_op \<Rightarrow> off_ty \<Rightarrow> reg_map \<Rightarrow> mem \<Rightarrow> mem option" where
+"eval_store chk dst sop off rs mem = (
+  case sop of (SOImm x) \<Rightarrow> None | SOReg x \<Rightarrow> 
+  let dv  =  (eval_reg dst rs) in (
+  let vm_addr :: u64 = (dv + (scast off)) in (  
+  let sv :: u64 = eval_snd_op_u64 sop rs in ( \<comment> \<open> TODO: sv is signed for imm and unsigned for src reg? \<close>
+  (storev chk mem (Vlong vm_addr) (memory_chunk_value_of_u64 chk sv))
+))))"
+
+
 definition eval_load :: "memory_chunk \<Rightarrow> dst_ty \<Rightarrow> src_ty \<Rightarrow> off_ty \<Rightarrow> reg_map \<Rightarrow> mem \<Rightarrow> reg_map option" where
 "eval_load chk dst sop off rs mem = (
   let sv :: u64 = eval_snd_op_u64 (SOReg sop) rs in (
@@ -148,15 +158,23 @@ fun sbpf_step :: "ebpf_asm \<Rightarrow> sbpf_state \<Rightarrow> sbpf_state" wh
         Some rs' \<Rightarrow> SBPF_OK (pc+1) rs' m
       ) |
     _ \<Rightarrow> SBPF_Err) |
-    BPF_JUMP cond dst snd_op off \<Rightarrow> 
-      (case snd_op of (SOImm x) \<Rightarrow> SBPF_Err | SOReg x \<Rightarrow> 
-      if eval_jmp cond dst snd_op rs then SBPF_OK (pc+1+scast off) rs m 
-      else SBPF_OK (pc + 1) rs m) | 
+
     BPF_LDX chk dst sop off \<Rightarrow> (
       case eval_load chk dst sop off rs m of
         None \<Rightarrow> SBPF_Err |
         Some rs' \<Rightarrow> SBPF_OK (pc+1) rs' m ) |
-    BPF_EXIT \<Rightarrow> SBPF_Success (rs BR0) |
+
+    BPF_JUMP cond dst snd_op off \<Rightarrow> 
+      (case snd_op of (SOImm x) \<Rightarrow> SBPF_Err | SOReg x \<Rightarrow> 
+      if eval_jmp cond dst snd_op rs then SBPF_OK (pc+1+scast off) rs m 
+      else SBPF_OK (pc + 1) rs m) | 
+
+    BPF_ST chk dst sop off \<Rightarrow> (
+      case eval_store chk dst sop off rs m of
+        None \<Rightarrow> SBPF_Err |
+        Some m' \<Rightarrow> SBPF_OK (pc+1) rs m' ) |
+    
+BPF_EXIT \<Rightarrow> SBPF_Success (rs BR0) |
     _ \<Rightarrow> SBPF_Err
 ))" |
 "sbpf_step prog _  = SBPF_Err" 
