theory/JITPer_store.thy
@@ -1,0 +1,401 @@
+theory JITPer_store
+
+imports
+  Main
+  rBPFCommType rBPFSyntax rBPFSem
+  x64Syntax x64Semantics x64Assembler
+  JITPer_aux
+
+begin
+
+lemma length_of_addrmode_instr:
+  assumes a0:"xins = (Pmov_rm R10 (Addrmode (Some R11) None 0) chk)" and
+  a1:"l_bin = x64_encode xins" and
+  a2:"chk = M64"
+  shows "length l_bin = 4"
+proof-
+  let "?a" = "(Addrmode (Some R11) None 0)"
+  let "?r1" =  "R10"
+  let "?c" = "chk"
+  have b1:"construct_rex_to_u8 (?c = M64) (and (u8_of_ireg ?r1) 0b1000 \<noteq> 0) False (and (u8_of_ireg R11) 0b1000 \<noteq> 0) \<noteq> 0x40"
+    using a2 by(unfold construct_rex_to_u8_def Let_def bitfield_insert_u8_def u8_of_bool_def,simp_all) 
+  have b3:"l_bin = (case ?a of Addrmode (Some rb) None dis \<Rightarrow> 
+      let (rex::u8) = ( construct_rex_to_u8 \<comment> \<open> WRXB \<close>
+        (?c = M64) \<comment> \<open> W \<close>
+        (and (u8_of_ireg ?r1) 0b1000 \<noteq> 0) \<comment> \<open> R \<close>
+        False \<comment> \<open> X \<close>
+        (and (u8_of_ireg rb) 0b1000 \<noteq> 0) \<comment> \<open> B \<close>
+        ) in
+        let (dis::u8) = scast dis in
+        let (rop::u8) = construct_modsib_to_u8 0b01 (u8_of_ireg ?r1) (u8_of_ireg rb) in
+        ([rex, 0x8b, rop, dis]))" using b1 using a0 a1 x64_encode_def a2 by(cases chk,simp_all)
+  thus ?thesis by simp
+qed
+
+
+(*lemma "\<exists> x y. ((scast(x::u8))::i8) + ((scast(y::u8))::i8) = (scast(x+y)::i8)"
+  by (metis (no_types, lifting) of_int_add scast_nop1)
+
+lemma "\<exists> x y. ((ucast(x::i8))::u8) + ((ucast(y::i8))::u8) = (ucast(x+y)::u8)"
+  by (metis add_0 unsigned_0)
+
+
+lemma cast_lemma3:"(x::u32) = (ucast(x::u32)::u32)"
+  by simp
+
+value "((scast (1::u64))::i64)"
+*)
+lemma cast_aux1:"\<forall> x y. ((scast(x::u64))::i64) + ((scast(y::u64))::i64) = (scast(x+y)::i64)"
+  by (metis (mono_tags, opaque_lifting) of_int_add of_int_sint scast_id scast_nop2 scast_scast_id(2))
+
+lemma cast_aux2:"(ucast ((scast(x::u64))::i64)::u64) = x"
+  using  scast_nop1
+  by (metis scast_scast_id(1) ucast_eq word_of_int_uint)
+
+lemma cast_lemma1:"(ucast(((scast(x::u64))::i64) + ((scast(y::u64))::i64))::u64) = x+y"
+  using cast_aux1 cast_aux2 by auto
+
+lemma store_mem_one_step1:
+ assumes a0:"(SBPF_OK pc' rs' m') = sbpf_step prog (SBPF_OK pc rs m)" and
+    a1:"xst = (Next xpc xrs xm)" and
+    a2:"match_state (SBPF_OK pc rs m) (pc,xst)" and
+    a3:"prog \<noteq> [] \<and> unat pc < length prog \<and> unat pc \<ge> 0" and
+    a4:"prog!(unat pc) = BPF_ST chk dst (SOReg src) off" and
+    a5:"chk = M64"
+  shows "storev chk xm (Vlong (scast off + xrs (IR (bpf_to_x64_reg dst)))) (Vlong (xrs (IR (bpf_to_x64_reg src)))) \<noteq> None"
+proof-
+
+  have "\<exists> xm'. Some xm' = (let off = (xrs (IR (bpf_to_x64_reg dst)) + scast off); l = u8_list_of_u64 (ucast (xrs (IR (bpf_to_x64_reg src)))) in
+               Some  (\<lambda> x i. if x = 0 \<and> i = (uint off)    then Some (l!(0)) else
+                   if x = 0 \<and> i = (uint off)+1  then Some (l!(1)) else
+                   if x = 0 \<and> i = (uint off)+2  then Some (l!(2)) else
+                   if x = 0 \<and> i = (uint off)+3  then Some (l!(3)) else
+                   if x = 0 \<and> i = (uint off)+4  then Some (l!(4)) else
+                   if x = 0 \<and> i = (uint off)+5  then Some (l!(5)) else
+                   if x = 0 \<and> i = (uint off)+6  then Some (l!(6)) else
+                   if x = 0 \<and> i = (uint off)+7  then Some (l!(7)) else
+                      m 0 i))" 
+    using storev_def apply(cases "(xrs (IR (bpf_to_x64_reg src)))",simp_all)
+    subgoal for n by metis done
+  then obtain xm' where "Some xm' = (let off = (xrs (IR (bpf_to_x64_reg dst)) + scast off); l = u8_list_of_u64 (ucast (xrs (IR (bpf_to_x64_reg src)))) in
+               Some (\<lambda> x i. if x = 0 \<and> i = (uint off)    then Some (l!(0)) else
+                   if x = 0 \<and> i = (uint off)+1  then Some (l!(1)) else
+                   if x = 0 \<and> i = (uint off)+2  then Some (l!(2)) else
+                   if x = 0 \<and> i = (uint off)+3  then Some (l!(3)) else
+                   if x = 0 \<and> i = (uint off)+4  then Some (l!(4)) else
+                   if x = 0 \<and> i = (uint off)+5  then Some (l!(5)) else
+                   if x = 0 \<and> i = (uint off)+6  then Some (l!(6)) else
+                   if x = 0 \<and> i = (uint off)+7  then Some (l!(7)) else
+                      m 0 i))" by auto
+  thus ?thesis using storev_def 
+    by (metis (no_types, lifting) a5 memory_chunk.simps(16) option.distinct(1) val.simps(40))
+qed
+
+lemma store_mem_one_step2:
+    "(SBPF_OK pc' rs' m') = sbpf_step prog (SBPF_OK pc rs m) \<Longrightarrow>
+    xst = (Next xpc xrs xm) \<Longrightarrow>
+    match_state (SBPF_OK pc rs m) (pc,xst) \<Longrightarrow>
+    prog \<noteq> [] \<and> unat pc < length prog \<and> unat pc \<ge> 0 \<Longrightarrow>
+    prog!(unat pc) = BPF_ST chk dst (SOReg src) off  \<Longrightarrow>
+    storev chk xm (Vlong (scast off + xrs (IR (bpf_to_x64_reg dst)))) (Vlong (xrs (IR (bpf_to_x64_reg src)))) = Some a \<Longrightarrow>
+    match_reg rs' (\<lambda>a::preg. if a = IR REG_OTHER_SCRATCH then xrs (IR (bpf_to_x64_reg src)) else if a = IR REG_SCRATCH then scast off + xrs (IR (bpf_to_x64_reg dst)) else if a = IR REG_SCRATCH then scast off else xrs a)"
+  apply (simp add: match_state_def match_reg_def eval_load_def)
+  using bpf_to_x64_reg_corr reg_r11_consist reg_rsp_consist reg_r10_consist
+  by (metis option.case_eq_if sbpf_state.inject(1) sbpf_state.simps(6))
+
+
+lemma store_mem_one_step3:
+  assumes a0:"(SBPF_OK pc' rs' m') = sbpf_step prog (SBPF_OK pc rs m)" and
+    a1:"xst = (Next xpc xrs xm)" and
+    a2:"match_state (SBPF_OK pc rs m) (pc,xst)" and
+    a3:"prog \<noteq> [] \<and> unat pc < length prog \<and> unat pc \<ge> 0" and
+    a4:"prog!(unat pc) =  BPF_ST chk dst (SOReg src) off" and
+    a5:"storev chk xm (Vlong (scast off + xrs (IR (bpf_to_x64_reg dst)))) (Vlong (xrs (IR (bpf_to_x64_reg src)))) = Some xm'" 
+    shows "match_mem m' xm' "
+proof-        
+  have c_old_mem_eqiv:"\<forall> mc addr v. (Mem.loadv mc m (Vlong addr) = Some v) \<longrightarrow> (Mem.loadv mc xm (Vlong addr) = Some v)"
+    using a1 a2 match_state_def match_mem_def by simp
+  have c_src_eqiv:"xrs (IR (bpf_to_x64_reg src)) = rs (src)" using match_state_def match_reg_def a2 a1 by simp
+  have c_dst_eqiv:"xrs (IR (bpf_to_x64_reg dst)) = rs (dst)" using match_state_def match_reg_def a2 a1 by simp
+
+  have b0:" Some m' = (let dv = (eval_reg dst rs) in (
+  let vm_addr  = (dv + (scast off)) in (  
+  let sv :: u64 = eval_snd_op_u64 (SOReg src) rs in (
+  (storev chk m (Vlong vm_addr) (memory_chunk_value_of_u64 chk sv))))))" using a0 a3 a4 eval_store_def
+    by (smt (verit) bpf_instruction.case(3) option.case_eq_if option.collapse sbpf_state.inject(1) sbpf_state.simps(6) sbpf_step.elims snd_op.simps(6))
+    
+  
+  let "?x_addr" = "(xrs (IR (bpf_to_x64_reg dst)) + scast off)"
+
+  let "?b_addr" = "((rs dst) + (scast off))"
+
+  have addr_eqiv: "?x_addr = ?b_addr"
+    using c_dst_eqiv by force
+
+  let "?x_val" = "xrs (IR (bpf_to_x64_reg src))"
+
+  let "?b_val" = "rs src"
+
+  have c_upate_m_to_m':"Some m' = storev chk m (Vlong ?b_addr) (memory_chunk_value_of_u64 chk (rs src) )"  using b0 eval_reg_def by force
+
+
+  have d_old_places_of_m: "\<forall> addr v chk m'. ((uint ?b_addr) + memory_chunk_to_byte_int chk < (uint addr)) \<or>
+  ((uint addr) + memory_chunk_to_byte_int chk < (uint ?b_addr)) \<longrightarrow> 
+  Some m' = storev chk m (Vlong ?b_addr) (memory_chunk_value_of_u64 chk (rs src) ) \<longrightarrow>
+  loadv chk m (Vlong addr) = loadv chk m' (Vlong addr)"
+    using c_upate_m_to_m' storev_def store_load_other_vlong2 
+    by (smt (verit, ccfv_SIG) not_Some_eq store_load_other_vlong)
+
+  have d_old_places_of_xm:"\<forall> addr v chk xm'. ((uint ?x_addr) + memory_chunk_to_byte_int chk < (uint addr)) \<or>
+  ((uint addr) + memory_chunk_to_byte_int chk < (uint ?x_addr)) \<longrightarrow> 
+   storev chk xm (Vlong (scast off + xrs (IR (bpf_to_x64_reg dst)))) (Vlong (xrs (IR (bpf_to_x64_reg src)))) = Some xm' \<longrightarrow>
+  loadv chk xm (Vlong addr) = loadv chk xm' (Vlong addr)" using store_load_other_vlong2 c_upate_m_to_m'
+    by (smt (z3) add.commute loadv_def option.case_eq_if option_val_of_u64_def store_load_other_vlong val.simps(40))
+
+
+  have d_old_places_eqiv_aux:"\<forall> addr v chk m' xm'. ((uint ?x_addr) + memory_chunk_to_byte_int chk < (uint addr)) \<or>
+  ((uint addr) + memory_chunk_to_byte_int chk < (uint ?x_addr)) \<longrightarrow> 
+     Some m' = storev chk m (Vlong ?b_addr) (memory_chunk_value_of_u64 chk (rs src) ) \<longrightarrow>
+     Some xm' = storev chk xm (Vlong ?x_addr) (Vlong (xrs (IR (bpf_to_x64_reg src))))  \<longrightarrow> 
+   (Mem.loadv chk m' (Vlong addr) = Some v) \<longrightarrow> (Mem.loadv chk xm' (Vlong addr) = Some v)" 
+    using d_old_places_of_m d_old_places_of_xm c_old_mem_eqiv c_dst_eqiv c_src_eqiv a5
+    by (smt (verit, ccfv_SIG) store_load_other_vlong)
+
+
+  have d_old_places_eqiv:"\<forall> addr v. ((uint ?x_addr) + memory_chunk_to_byte_int chk < (uint addr)) \<or>
+  ((uint addr) + memory_chunk_to_byte_int chk < (uint ?x_addr)) \<longrightarrow> 
+     Some m' = storev chk m (Vlong ?x_addr) (memory_chunk_value_of_u64 chk (rs src) ) \<longrightarrow>
+     Some xm' = storev chk xm (Vlong ?x_addr) (Vlong (xrs (IR (bpf_to_x64_reg src))))  \<longrightarrow> 
+   (Mem.loadv chk m' (Vlong addr) = Some v) \<longrightarrow> (Mem.loadv chk xm' (Vlong addr) = Some v)" 
+    using d_old_places_eqiv_aux addr_eqiv by simp
+
+
+ have d_new_places_eqiv_aux1:"loadv chk xm' (Vlong ?x_addr) = loadv chk m' (Vlong ?b_addr)" 
+    (*using store_load_consistency_m64 store_load_consistency_m32 store_load_consistency_m16 store_load_consistency_m8*)
+    using c_upate_m_to_m' c_dst_eqiv c_src_eqiv a5 storev_def apply(cases chk,simp_all) 
+    using store_load_consistency_m64 apply (simp add: storev_def)
+    by (simp add: add.commute memory_chunk_value_of_u64_def) 
+
+  have d_new_places_eqiv_aux2:"\<forall> v. (Mem.loadv chk xm' (Vlong ?x_addr) = Some v) \<longrightarrow> (Mem.loadv chk m' (Vlong ?x_addr) = Some v)"
+    using d_new_places_eqiv_aux1 addr_eqiv by simp
+
+  have d_new_places_eqiv:"\<forall> addr v. 
+  ((uint ?x_addr - memory_chunk_to_byte_int chk) \<le> (uint addr)) \<and> ((uint addr) \<le> (uint ?x_addr) + memory_chunk_to_byte_int chk) \<longrightarrow>
+  (Mem.loadv chk m' (Vlong addr) = Some v) \<longrightarrow> (Mem.loadv chk xm' (Vlong addr) = Some v)" 
+    using d_new_places_eqiv_aux1 c_dst_eqiv sorry
+ 
+  have d_places_eqiv:"\<forall> addr v.
+     Some m' = storev chk m (Vlong ?b_addr) (memory_chunk_value_of_u64 chk (rs src) ) \<longrightarrow>
+     Some xm' = storev chk xm (Vlong ?x_addr) (Vlong (xrs (IR (bpf_to_x64_reg src))))  \<longrightarrow> 
+   (Mem.loadv chk m' (Vlong addr) = Some v) \<longrightarrow> (Mem.loadv chk xm' (Vlong addr) = Some v)" 
+    using d_old_places_eqiv d_new_places_eqiv 
+    by (smt (verit, ccfv_SIG) d_old_places_eqiv_aux)
+ 
+  have "\<forall> addr v. (Mem.loadv chk m' (Vlong addr) = Some v) \<longrightarrow> (Mem.loadv chk xm' (Vlong addr) = Some v)"
+    using d_places_eqiv d_old_places_eqiv c_upate_m_to_m' a5 
+    by (simp add: add.commute)
+
+  have "\<forall> addr v chk. (Mem.loadv chk m' (Vlong addr) = Some v) \<longrightarrow> (Mem.loadv chk xm' (Vlong addr) = Some v)" sorry
+
+  thus ?thesis using match_mem_def by presburger
+qed
+
+
+
+value "uint (0::u64)"
+
+value "uint (1::u64)"
+
+
+lemma store_mem_one_step4:
+  "(SBPF_OK pc' rs' m') = sbpf_step prog (SBPF_OK pc rs m) \<Longrightarrow>
+    xst = (Next xpc xrs xm) \<Longrightarrow>
+    match_state (SBPF_OK pc rs m) (pc,xst) \<Longrightarrow>
+    prog \<noteq> [] \<and> unat pc < length prog \<and> unat pc \<ge> 0 \<Longrightarrow>
+    prog!(unat pc) =  BPF_ST chk dst (SOReg src) off   \<Longrightarrow>
+    storev chk xm (Vlong (scast off + xrs (IR (bpf_to_x64_reg dst)))) (Vlong (xrs (IR (bpf_to_x64_reg src)))) = Some a \<Longrightarrow>
+    match_stack(\<lambda>a::preg. if a = IR REG_OTHER_SCRATCH then xrs (IR (bpf_to_x64_reg src)) else if a = IR REG_SCRATCH then scast off + xrs (IR (bpf_to_x64_reg dst)) else if a = IR REG_SCRATCH then scast off else xrs a)"
+  by (simp add: match_state_def match_stack_def eval_alu_def eval_reg_def)
+ 
+
+lemma store_mem_one_step:
+  "(SBPF_OK pc' rs' m') = sbpf_step prog (SBPF_OK pc rs m) \<Longrightarrow>
+    xst = (Next xpc xrs xm) \<Longrightarrow>
+    match_state (SBPF_OK pc rs m) (pc,xst) \<Longrightarrow>
+    prog \<noteq> [] \<and> unat pc < length prog \<and> unat pc \<ge> 0 \<Longrightarrow>
+    prog!(unat pc) =  BPF_ST chk dst (SOReg src) off   \<Longrightarrow>
+    storev chk xm (Vlong (scast off + xrs (IR (bpf_to_x64_reg dst)))) (Vlong (xrs (IR (bpf_to_x64_reg src)))) = Some a \<Longrightarrow>
+    match_reg rs' (\<lambda>a::preg. if a = IR REG_OTHER_SCRATCH then xrs (IR (bpf_to_x64_reg src)) else if a = IR REG_SCRATCH then scast off + xrs (IR (bpf_to_x64_reg dst)) else if a = IR REG_SCRATCH then scast off else xrs a) \<and>
+    match_mem m' a \<and> match_stack(\<lambda>a::preg. if a = IR REG_OTHER_SCRATCH then xrs (IR (bpf_to_x64_reg src)) else if a = IR REG_SCRATCH then scast off + xrs (IR (bpf_to_x64_reg dst)) else if a = IR REG_SCRATCH then scast off else xrs a)"
+  using store_mem_one_step2 store_mem_one_step3 store_mem_one_step4 by simp
+
+
+lemma store_one_step1:
+ assumes a0:"s' = sbpf_step prog s" and
+  a1:"s = (SBPF_OK pc rs m)" and
+  a2:"s' = (SBPF_OK pc' rs' m')" and
+  a3:"xst = (Next xpc xrs xm)" and
+  a4:"match_state s (pc,xst)" and
+  a5:"jitper prog = Some x64_prog" and                      
+  a6:"prog \<noteq> [] \<and> unat pc < length prog \<and> unat pc \<ge> 0" and
+  a8:"prog!(unat pc) = BPF_ST chk dst (SOReg src) off" and
+  a9:"chk = M64"
+shows "\<exists> xst'. x64_sem1 1 x64_prog (pc,xst) = (pc',xst') \<and> 
+  match_state s' (pc',xst')"
+(* 1. as BPF_ADD generates a single list of jited x64 assembly, so we only need one step  *)
+  apply(subgoal_tac "\<exists>xst'::outcome. one_step x64_prog (pc, xst) = (pc', xst') \<and> match_state s' (pc', xst')")
+  subgoal
+    by auto
+  subgoal
+    apply (unfold one_step_def Let_def)
+(* 2. according to the code structure of JITPer, removing the first case statement *)
+    apply(subgoal_tac "x64_prog ! unat (fst (pc, xst)) = the (per_jit_store_reg64 dst src chk off)")
+     prefer 2
+    subgoal
+      using a5 a6 a8 aux5 per_jit_ins_def by fastforce
+    subgoal
+      apply (subgoal_tac "the (per_jit_store_reg64 dst src chk off) = (4, 0, x64_encode (Pmovq_ri R11 (scast off))@x64_encode (Paddq_rr R11 (bpf_to_x64_reg dst))@
+    x64_encode (Pmovq_rr R10 (bpf_to_x64_reg src))@x64_encode (Pmov_rm R10 (Addrmode (Some R11) None 0) chk))")
+       prefer 2
+      subgoal by (simp add: per_jit_store_reg64_def Let_def)
+      apply (subgoal_tac "(x64_encode (Pmovq_ri R11 (scast off))@x64_encode (Paddq_rr R11 (bpf_to_x64_reg dst))@
+    x64_encode (Pmovq_rr R10 (bpf_to_x64_reg src))@x64_encode (Pmov_rm R10 (Addrmode (Some R11) None 0) chk)) !1 \<noteq> 0x39")
+       prefer 2
+      subgoal apply(unfold x64_encode_def) 
+        apply(cases "Pmovq_ri REG_SCRATCH (scast off)",simp_all)
+        using x64_encode_def construct_rex_to_u8_def bitfield_insert_u8_def Let_def
+        by simp
+      subgoal
+        unfolding a3
+        apply simp
+        apply (erule subst)
+        apply (erule subst)
+(* 3. here we get a simplified version, next step is to run the 6 x64 assembly one by one *)
+(* 3.1 *)
+        apply (subgoal_tac "Suc 3 = (4::nat)") prefer 2 subgoal by simp
+        apply (erule subst [of _ 4])
+        apply (simp only: x64_sem.simps)
+        apply simp
+(* 3.1.1 using consistency to get x64 assembly *)
+        apply (subgoal_tac "x64_decode (0::nat)
+            (x64_encode (Pmovq_ri R11 (scast off))@x64_encode (Paddq_rr R11 (bpf_to_x64_reg dst))@
+    x64_encode (Pmovq_rr R10 (bpf_to_x64_reg src))@x64_encode (Pmov_rm R10 (Addrmode (Some R11) None 0) chk))
+            = Some (10, Pmovq_ri REG_SCRATCH (scast off))")
+         prefer 2
+        subgoal
+          apply (rule_tac l_bin = "x64_encode (Pmovq_ri REG_SCRATCH (scast off))" in x64_encode_decode_consistency)
+          subgoal using list_in_list_prop
+            using list_in_list_concat by blast
+          subgoal by simp
+          subgoal using x64_encode_def construct_rex_to_u8_def bitfield_insert_u8_def Let_def u8_list_of_u64_def
+            by auto
+          done
+        apply simp
+        apply (erule subst)
+        apply (simp add: exec_instr_def)
+(* 3.2 *)
+        apply (subgoal_tac "Suc 2 = (3::nat)") prefer 2 subgoal by simp
+        apply (erule subst [of _ 3])
+        apply (simp only: x64_sem.simps)
+        apply simp
+        apply (subgoal_tac "x64_decode (10::nat)
+            (x64_encode (Pmovq_ri R11 (scast off))@x64_encode (Paddq_rr R11 (bpf_to_x64_reg dst))@
+    x64_encode (Pmovq_rr R10 (bpf_to_x64_reg src))@x64_encode (Pmov_rm R10 (Addrmode (Some R11) None 0) chk))
+            = Some (3, Paddq_rr R11 (bpf_to_x64_reg dst))")
+         prefer 2
+(* this is necessary for later list_in_list_prop_aux2 *)
+        apply (subgoal_tac "length (x64_encode (Pmovq_ri REG_SCRATCH (scast off))) = 10")
+         prefer 2 subgoal using x64_encode_def construct_rex_to_u8_def bitfield_insert_u8_def Let_def u8_list_of_u64_def by auto
+        subgoal
+          apply (rule_tac l_bin = "x64_encode (Paddq_rr R11 (bpf_to_x64_reg dst))" in x64_encode_decode_consistency)
+          subgoal using list_in_list_prop_aux2
+            by metis 
+          subgoal by simp
+          subgoal apply (erule subst) 
+            using x64_encode_def construct_rex_to_u8_def bitfield_insert_u8_def Let_def
+            by fastforce
+          done
+        apply simp
+        apply (erule subst)
+        apply (simp add: exec_instr_def)
+        apply(subgoal_tac "bpf_to_x64_reg dst \<noteq> REG_SCRATCH") 
+        prefer 2 using reg_r11_consist apply blast
+         apply (rule conjI)
+          apply (rule impI)
+          apply simp
+         apply (rule impI)
+         apply (simp add: exec_instr_def Let_def)
+
+(* 3.3 *)
+        apply (subgoal_tac "Suc 1 = (2::nat)") prefer 2 subgoal by simp
+        apply (erule_tac subst [of _ 2])
+        apply (simp only: x64_sem.simps)
+        (*apply simp*)
+(* using consistency to get x64 assembly *)
+        apply (subgoal_tac "x64_decode (13::nat)
+            (x64_encode (Pmovq_ri R11 (scast off))@x64_encode (Paddq_rr R11 (bpf_to_x64_reg dst))@
+    x64_encode (Pmovq_rr R10 (bpf_to_x64_reg src))@x64_encode (Pmov_rm R10 (Addrmode (Some R11) None 0) chk))
+            = Some (3, Pmovq_rr R10 (bpf_to_x64_reg src))")
+         prefer 2
+(* this is necessary for later list_in_list_prop_aux2 *)
+        apply (subgoal_tac "length ((x64_encode (Pmovq_ri R11 (scast off))@x64_encode (Paddq_rr R11 (bpf_to_x64_reg dst)))) = 13")
+         prefer 2 subgoal using x64_encode_def construct_rex_to_u8_def bitfield_insert_u8_def Let_def u8_list_of_u64_def by auto
+        subgoal
+          apply (rule_tac l_bin = "x64_encode (Pmovq_rr R10 (bpf_to_x64_reg src))" in x64_encode_decode_consistency)
+          subgoal using list_in_list_prop_aux2
+            by (metis (no_types, opaque_lifting) append_eq_append_conv2)
+          subgoal by simp
+          subgoal using x64_encode_def construct_rex_to_u8_def bitfield_insert_u8_def Let_def by fastforce 
+          done 
+        apply simp
+        apply (erule subst)
+        apply (simp add: exec_instr_def Let_def)
+        apply(subgoal_tac "bpf_to_x64_reg src \<noteq> REG_SCRATCH") 
+         prefer 2 subgoal using reg_r11_consist by blast
+         apply (rule conjI)
+         apply (rule impI)
+         apply simp
+        apply(rule impI)
+
+        apply (subgoal_tac "Suc 0 = (1::nat)") prefer 2 subgoal by simp
+        apply (erule_tac subst [of _ 1])
+        apply (simp only: x64_sem.simps)
+        (*apply simp*)
+(* using consistency to get x64 assembly *)
+        apply (subgoal_tac "x64_decode (16::nat)
+            (x64_encode (Pmovq_ri R11 (scast off))@x64_encode (Paddq_rr R11 (bpf_to_x64_reg dst))@
+    x64_encode (Pmovq_rr R10 (bpf_to_x64_reg src))@x64_encode (Pmov_rm R10 (Addrmode (Some R11) None 0) chk))
+            = Some (4, Pmov_rm R10 (Addrmode (Some R11) None 0) chk)")
+         prefer 2
+(* this is necessary for later list_in_list_prop_aux2 *)
+        apply (subgoal_tac "length (x64_encode (Pmovq_ri R11 (scast off))@x64_encode (Paddq_rr R11 (bpf_to_x64_reg dst))@
+    x64_encode (Pmovq_rr R10 (bpf_to_x64_reg src))) = 16")
+         prefer 2 subgoal using x64_encode_def construct_rex_to_u8_def bitfield_insert_u8_def Let_def u8_list_of_u64_def by auto
+        subgoal
+          apply (rule_tac l_bin = "x64_encode (Pmov_rm R10 (Addrmode (Some R11) None 0) chk)" in x64_encode_decode_consistency)
+          subgoal using list_in_list_prop_aux2
+            by (metis (no_types, opaque_lifting) append_eq_append_conv2)
+          subgoal by simp
+          subgoal using length_of_addrmode_instr a9 by simp done
+        apply simp
+        apply (erule subst)
+        apply (simp add: exec_instr_def exec_store_def eval_addrmode64_def Let_def)
+        apply(subgoal_tac "bpf_to_x64_reg src \<noteq> REG_SCRATCH") 
+         prefer 2 subgoal using reg_r11_consist by blast
+         apply (rule conjI)
+(* 4. now we get exec_instr (one step of x64 add assembly), we prove the \<and>, first left, then right *)
+        subgoal
+          using a0 a1 a2 a5 a6 a8 corr_pc_aux2 insert_iff prod_cases3 by metis
+        unfolding a1 a2
+(* 4.1  match_reg *)
+         apply (simp add: match_state_def)
+         apply(cases "storev chk xm (Vlong (scast off + xrs (IR (bpf_to_x64_reg dst)))) (Vlong (xrs (IR (bpf_to_x64_reg src))))",simp_all)
+        subgoal using store_mem_one_step1 a0 a1 a2 a3 a4 a5 a6 a8 a9 by metis 
+        subgoal for m' using store_mem_one_step a9 a0 a1 a2 a3 a4 a5 a6 a8 
+          apply simp
+          done
+        done
+      done
+    done
+  done
+end
